@prefix swe:   <urn:x-gsml-rdf:types> .
@prefix sf:    <http://def.seegrid.csiro.au/isotc211/iso19156/2011/sampling> .
@prefix anzsmlss: <https://anzsoil.org/ont/anzsoilml-sample/> .
@prefix rdf:   <http://www.w3.org/1999/02/22-rdf-syntax-ns#> .
@prefix owl:   <http://www.w3.org/2002/07/owl#> .
@prefix xsd:   <http://www.w3.org/2001/XMLSchema#> .
@prefix skos:  <http://www.w3.org/2004/02/skos/core#> .
@prefix rdfs:  <http://www.w3.org/2000/01/rdf-schema#> .

anzsmlss:SoilSpecimen
        a                owl:Class ;
        rdfs:subClassOf  sf:SF_Specimen ;
        rdfs:subClassOf  [ a                  owl:Restriction ;
                           owl:allValuesFrom  xsd:boolean ;
                           owl:onProperty     anzsmlss:coarseFragmentsPresent
                         ] ;
        rdfs:subClassOf  [ a                  owl:Restriction ;
                           owl:allValuesFrom  xsd:boolean ;
                           owl:onProperty     anzsmlss:coarseFragmentsPresent
                         ] ;
        skos:definition  "A specialisation of SF_Specimen to capture archived specimens. \r\nNatSoil archive indicates whether there is a coarse fraction (>2mm) present in the specimen."@en .

anzsmlss:coarseFragmentsPresent
        a                owl:DatatypeProperty ;
        rdfs:range       xsd:boolean ;
        skos:definition  "Presence or absence of coarse fragment sample >2mm"@en .

<https://anzsoil.org/ont/anzsoilml-sample>
        a                owl:Ontology ;
        owl:imports      <http://def.seegrid.csiro.au/isotc211/iso19156/2011/sampling.ttl> , <http://schemas.geosciml.org/rdf/types.ttl> ;
        owl:versionIRI   "https://soilmlie.org/def/soilml#/anzsmlss/1.0.0" ;
        owl:versionInfo  "1.0.0" ;
        skos:definition  "Application Schema for soil sampling, soil specimens and related observations"@en .

anzsmlss:lowerDepth  a   owl:ObjectProperty ;
        rdfs:range       swe:Quantity ;
        skos:definition  "To specify the upper and lower depths that the sample was taken from"@en .

anzsmlss:SoilSample  a   owl:Class ;
        rdfs:subClassOf  [ a                  owl:Restriction ;
                           owl:allValuesFrom  swe:Quantity ;
                           owl:onProperty     anzsmlss:upperDepth
                         ] ;
        rdfs:subClassOf  [ a                  owl:Restriction ;
                           owl:allValuesFrom  swe:Quantity ;
                           owl:onProperty     anzsmlss:lowerDepth
                         ] ;
        skos:definition  "A specialisation of SF_SpatialSamplingFeature for soil sampling features."@en , "A specialisation of SF_SpatialSamplingFeature to allow the depth at which the sample was taken and the size of the sample."@en .

anzsmlss:upperDepth  a   owl:ObjectProperty ;
        rdfs:range       swe:Quantity ;
        skos:definition  "To specify the upper and lower depths that the sample was taken from"@en .
